hax-lib/proof-libs/fstar/core/Alloc.Collections.Btree.Map.fsti
@@ -3,7 +3,366 @@ module Alloc.Collections.Btree.Map
 open FStar.Mul
 open Rust_primitives
 
+type t_BTreeMap (v_K: Type0) (v_V: Type0) (v_A: Type0) =
+  | BTreeMap : Rust_primitives.Sequence.t_Seq (v_K & v_V) -> Core_models.Marker.t_PhantomData v_A
+    -> t_BTreeMap v_K v_V v_A
+
 /// See [`std::collections::btree_map::UnorderedKeyError`]: the error
 /// `CursorMut::insert_before`/`insert_after` return. The cursor API
 /// itself is not modeled, so nothing here produces one.
 type t_UnorderedKeyError = | UnorderedKeyError : t_UnorderedKeyError
+
+/// See [`std::collections::btree_map::Iter`]
+type t_Iter (v_K: Type0) (v_V: Type0) =
+  | Iter : Rust_primitives.Sequence.t_Seq (v_K & v_V) -> t_Iter v_K v_V
+
+/// See [`std::collections::btree_map::Keys`]
+type t_Keys (v_K: Type0) (v_V: Type0) =
+  | Keys : Rust_primitives.Sequence.t_Seq v_K -> Core_models.Marker.t_PhantomData v_V
+    -> t_Keys v_K v_V
+
+/// See [`std::collections::btree_map::Values`]
+type t_Values (v_K: Type0) (v_V: Type0) =
+  | Values : Rust_primitives.Sequence.t_Seq v_V -> Core_models.Marker.t_PhantomData v_K
+    -> t_Values v_K v_V
+
+/// See [`std::collections::btree_map::IntoKeys`]
+type t_IntoKeys (v_K: Type0) (v_V: Type0) (v_A: Type0) =
+  | IntoKeys : Rust_primitives.Sequence.t_Seq (v_K & v_V) -> Core_models.Marker.t_PhantomData v_A
+    -> t_IntoKeys v_K v_V v_A
+
+/// See [`std::collections::btree_map::IntoValues`]
+type t_IntoValues (v_K: Type0) (v_V: Type0) (v_A: Type0) =
+  | IntoValues : Rust_primitives.Sequence.t_Seq (v_K & v_V) -> Core_models.Marker.t_PhantomData v_A
+    -> t_IntoValues v_K v_V v_A
+
+[@@ FStar.Tactics.Typeclasses.tcinstance]
+let impl (#v_K #v_V: Type0) : Core_models.Iter.Traits.Iterator.t_Iterator (t_Iter v_K v_V) =
+  {
+    f_Item = (v_K & v_V);
+    f_next_pre = (fun (self: t_Iter v_K v_V) -> true);
+    f_next_post
+    =
+    (fun
+        (self: t_Iter v_K v_V)
+        (out1: (t_Iter v_K v_V & Core_models.Option.t_Option (v_K & v_V)))
+        ->
+        true);
+    f_next
+    =
+    fun (self: t_Iter v_K v_V) ->
+      let (self: t_Iter v_K v_V), (hax_temp_output: Core_models.Option.t_Option (v_K & v_V)) =
+        if (Rust_primitives.Sequence.seq_len #(v_K & v_V) self._0 <: usize) =. mk_usize 0
+        then
+          self, (Core_models.Option.Option_None <: Core_models.Option.t_Option (v_K & v_V))
+          <:
+          (t_Iter v_K v_V & Core_models.Option.t_Option (v_K & v_V))
+        else
+          let (tmp0: Rust_primitives.Sequence.t_Seq (v_K & v_V)), (out: (v_K & v_V)) =
+            Rust_primitives.Sequence.seq_remove #(v_K & v_V) self._0 (mk_usize 0)
+          in
+          let self:t_Iter v_K v_V = { self with _0 = tmp0 } <: t_Iter v_K v_V in
+          let p:(v_K & v_V) = out in
+          self,
+          (Core_models.Option.Option_Some (p._1, p._2 <: (v_K & v_V))
+            <:
+            Core_models.Option.t_Option (v_K & v_V))
+          <:
+          (t_Iter v_K v_V & Core_models.Option.t_Option (v_K & v_V))
+      in
+      self, hax_temp_output <: (t_Iter v_K v_V & Core_models.Option.t_Option (v_K & v_V))
+  }
+
+[@@ FStar.Tactics.Typeclasses.tcinstance]
+let impl_1 (#v_K #v_V: Type0) : Core_models.Iter.Traits.Iterator.t_Iterator (t_Keys v_K v_V) =
+  {
+    f_Item = v_K;
+    f_next_pre = (fun (self: t_Keys v_K v_V) -> true);
+    f_next_post
+    =
+    (fun (self: t_Keys v_K v_V) (out1: (t_Keys v_K v_V & Core_models.Option.t_Option v_K)) -> true);
+    f_next
+    =
+    fun (self: t_Keys v_K v_V) ->
+      let (self: t_Keys v_K v_V), (hax_temp_output: Core_models.Option.t_Option v_K) =
+        if (Rust_primitives.Sequence.seq_len #v_K self._0 <: usize) =. mk_usize 0
+        then
+          self, (Core_models.Option.Option_None <: Core_models.Option.t_Option v_K)
+          <:
+          (t_Keys v_K v_V & Core_models.Option.t_Option v_K)
+        else
+          let (tmp0: Rust_primitives.Sequence.t_Seq v_K), (out: v_K) =
+            Rust_primitives.Sequence.seq_remove #v_K self._0 (mk_usize 0)
+          in
+          let self:t_Keys v_K v_V = { self with _0 = tmp0 } <: t_Keys v_K v_V in
+          self, (Core_models.Option.Option_Some out <: Core_models.Option.t_Option v_K)
+          <:
+          (t_Keys v_K v_V & Core_models.Option.t_Option v_K)
+      in
+      self, hax_temp_output <: (t_Keys v_K v_V & Core_models.Option.t_Option v_K)
+  }
+
+[@@ FStar.Tactics.Typeclasses.tcinstance]
+let impl_2 (#v_K #v_V: Type0) : Core_models.Iter.Traits.Iterator.t_Iterator (t_Values v_K v_V) =
+  {
+    f_Item = v_V;
+    f_next_pre = (fun (self: t_Values v_K v_V) -> true);
+    f_next_post
+    =
+    (fun (self: t_Values v_K v_V) (out1: (t_Values v_K v_V & Core_models.Option.t_Option v_V)) ->
+        true);
+    f_next
+    =
+    fun (self: t_Values v_K v_V) ->
+      let (self: t_Values v_K v_V), (hax_temp_output: Core_models.Option.t_Option v_V) =
+        if (Rust_primitives.Sequence.seq_len #v_V self._0 <: usize) =. mk_usize 0
+        then
+          self, (Core_models.Option.Option_None <: Core_models.Option.t_Option v_V)
+          <:
+          (t_Values v_K v_V & Core_models.Option.t_Option v_V)
+        else
+          let (tmp0: Rust_primitives.Sequence.t_Seq v_V), (out: v_V) =
+            Rust_primitives.Sequence.seq_remove #v_V self._0 (mk_usize 0)
+          in
+          let self:t_Values v_K v_V = { self with _0 = tmp0 } <: t_Values v_K v_V in
+          self, (Core_models.Option.Option_Some out <: Core_models.Option.t_Option v_V)
+          <:
+          (t_Values v_K v_V & Core_models.Option.t_Option v_V)
+      in
+      self, hax_temp_output <: (t_Values v_K v_V & Core_models.Option.t_Option v_V)
+  }
+
+[@@ FStar.Tactics.Typeclasses.tcinstance]
+let impl_3 (#v_K #v_V #v_A: Type0)
+    : Core_models.Iter.Traits.Iterator.t_Iterator (t_IntoKeys v_K v_V v_A) =
+  {
+    f_Item = v_K;
+    f_next_pre = (fun (self: t_IntoKeys v_K v_V v_A) -> true);
+    f_next_post
+    =
+    (fun
+        (self: t_IntoKeys v_K v_V v_A)
+        (out1: (t_IntoKeys v_K v_V v_A & Core_models.Option.t_Option v_K))
+        ->
+        true);
+    f_next
+    =
+    fun (self: t_IntoKeys v_K v_V v_A) ->
+      let (self: t_IntoKeys v_K v_V v_A), (hax_temp_output: Core_models.Option.t_Option v_K) =
+        if (Rust_primitives.Sequence.seq_len #(v_K & v_V) self._0 <: usize) =. mk_usize 0
+        then
+          self, (Core_models.Option.Option_None <: Core_models.Option.t_Option v_K)
+          <:
+          (t_IntoKeys v_K v_V v_A & Core_models.Option.t_Option v_K)
+        else
+          let (tmp0: Rust_primitives.Sequence.t_Seq (v_K & v_V)), (out: (v_K & v_V)) =
+            Rust_primitives.Sequence.seq_remove #(v_K & v_V) self._0 (mk_usize 0)
+          in
+          let self:t_IntoKeys v_K v_V v_A = { self with _0 = tmp0 } <: t_IntoKeys v_K v_V v_A in
+          self, (Core_models.Option.Option_Some out._1 <: Core_models.Option.t_Option v_K)
+          <:
+          (t_IntoKeys v_K v_V v_A & Core_models.Option.t_Option v_K)
+      in
+      self, hax_temp_output <: (t_IntoKeys v_K v_V v_A & Core_models.Option.t_Option v_K)
+  }
+
+[@@ FStar.Tactics.Typeclasses.tcinstance]
+let impl_4 (#v_K #v_V #v_A: Type0)
+    : Core_models.Iter.Traits.Iterator.t_Iterator (t_IntoValues v_K v_V v_A) =
+  {
+    f_Item = v_V;
+    f_next_pre = (fun (self: t_IntoValues v_K v_V v_A) -> true);
+    f_next_post
+    =
+    (fun
+        (self: t_IntoValues v_K v_V v_A)
+        (out1: (t_IntoValues v_K v_V v_A & Core_models.Option.t_Option v_V))
+        ->
+        true);
+    f_next
+    =
+    fun (self: t_IntoValues v_K v_V v_A) ->
+      let (self: t_IntoValues v_K v_V v_A), (hax_temp_output: Core_models.Option.t_Option v_V) =
+        if (Rust_primitives.Sequence.seq_len #(v_K & v_V) self._0 <: usize) =. mk_usize 0
+        then
+          self, (Core_models.Option.Option_None <: Core_models.Option.t_Option v_V)
+          <:
+          (t_IntoValues v_K v_V v_A & Core_models.Option.t_Option v_V)
+        else
+          let (tmp0: Rust_primitives.Sequence.t_Seq (v_K & v_V)), (out: (v_K & v_V)) =
+            Rust_primitives.Sequence.seq_remove #(v_K & v_V) self._0 (mk_usize 0)
+          in
+          let self:t_IntoValues v_K v_V v_A = { self with _0 = tmp0 } <: t_IntoValues v_K v_V v_A in
+          self, (Core_models.Option.Option_Some out._2 <: Core_models.Option.t_Option v_V)
+          <:
+          (t_IntoValues v_K v_V v_A & Core_models.Option.t_Option v_V)
+      in
+      self, hax_temp_output <: (t_IntoValues v_K v_V v_A & Core_models.Option.t_Option v_V)
+  }
+
+/// See [`std::collections::BTreeMap::new`]
+val impl_18__new: #v_K: Type0 -> #v_V: Type0 -> Prims.unit
+  -> Prims.Pure (t_BTreeMap v_K v_V Alloc.Alloc.t_Global) Prims.l_True (fun _ -> Prims.l_True)
+
+/// See [`std::collections::BTreeMap::clear`]
+val impl_19__clear (#v_K #v_V #v_A: Type0) (self: t_BTreeMap v_K v_V v_A)
+    : Prims.Pure (t_BTreeMap v_K v_V v_A) Prims.l_True (fun _ -> Prims.l_True)
+
+/// See [`std::collections::BTreeMap::new_in`]
+val impl_19__new_in (#v_K #v_V #v_A: Type0) (e_alloc: v_A)
+    : Prims.Pure (t_BTreeMap v_K v_V v_A) Prims.l_True (fun _ -> Prims.l_True)
+
+/// See [`std::collections::BTreeMap::get`]
+val impl_20__get
+      (#v_K #v_V #v_A #v_Q: Type0)
+      {| i0: Core_models.Borrow.t_Borrow v_K v_Q |}
+      {| i1: Core_models.Cmp.t_Ord v_K |}
+      {| i2: Core_models.Cmp.t_Ord v_Q |}
+      (self: t_BTreeMap v_K v_V v_A)
+      (key: v_Q)
+    : Prims.Pure (Core_models.Option.t_Option v_V) Prims.l_True (fun _ -> Prims.l_True)
+
+/// See [`std::collections::BTreeMap::get_key_value`]
+val impl_20__get_key_value
+      (#v_K #v_V #v_A #v_Q: Type0)
+      {| i0: Core_models.Borrow.t_Borrow v_K v_Q |}
+      {| i1: Core_models.Cmp.t_Ord v_K |}
+      {| i2: Core_models.Cmp.t_Ord v_Q |}
+      (self: t_BTreeMap v_K v_V v_A)
+      (k: v_Q)
+    : Prims.Pure (Core_models.Option.t_Option (v_K & v_V)) Prims.l_True (fun _ -> Prims.l_True)
+
+/// See [`std::collections::BTreeMap::contains_key`]
+val impl_20__contains_key
+      (#v_K #v_V #v_A #v_Q: Type0)
+      {| i0: Core_models.Borrow.t_Borrow v_K v_Q |}
+      {| i1: Core_models.Cmp.t_Ord v_K |}
+      {| i2: Core_models.Cmp.t_Ord v_Q |}
+      (self: t_BTreeMap v_K v_V v_A)
+      (key: v_Q)
+    : Prims.Pure bool Prims.l_True (fun _ -> Prims.l_True)
+
+/// See [`std::collections::BTreeMap::first_key_value`]
+val impl_20__first_key_value
+      (#v_K #v_V #v_A: Type0)
+      {| i0: Core_models.Cmp.t_Ord v_K |}
+      (self: t_BTreeMap v_K v_V v_A)
+    : Prims.Pure (Core_models.Option.t_Option (v_K & v_V)) Prims.l_True (fun _ -> Prims.l_True)
+
+/// See [`std::collections::BTreeMap::last_key_value`]
+val impl_20__last_key_value
+      (#v_K #v_V #v_A: Type0)
+      {| i0: Core_models.Cmp.t_Ord v_K |}
+      (self: t_BTreeMap v_K v_V v_A)
+    : Prims.Pure (Core_models.Option.t_Option (v_K & v_V)) Prims.l_True (fun _ -> Prims.l_True)
+
+/// See [`std::collections::BTreeMap::pop_first`]
+val impl_20__pop_first
+      (#v_K #v_V #v_A: Type0)
+      {| i0: Core_models.Cmp.t_Ord v_K |}
+      (self: t_BTreeMap v_K v_V v_A)
+    : Prims.Pure (t_BTreeMap v_K v_V v_A & Core_models.Option.t_Option (v_K & v_V))
+      Prims.l_True
+      (fun _ -> Prims.l_True)
+
+/// See [`std::collections::BTreeMap::pop_last`]
+val impl_20__pop_last
+      (#v_K #v_V #v_A: Type0)
+      {| i0: Core_models.Cmp.t_Ord v_K |}
+      (self: t_BTreeMap v_K v_V v_A)
+    : Prims.Pure (t_BTreeMap v_K v_V v_A & Core_models.Option.t_Option (v_K & v_V))
+      Prims.l_True
+      (fun _ -> Prims.l_True)
+
+/// See [`std::collections::BTreeMap::insert`]: on a key that is
+/// already present the *value* is replaced and the old one
+/// returned; the stored key is left alone, as in std.
+/// No `#[hax_lib::requires]` on the length here: that would need
+/// `#[hax_lib::attributes]` on the block, which moves it to the
+/// end of hax's impl numbering and so off index 20. `seq_insert`
+/// carries the bound instead.
+val impl_20__insert
+      (#v_K #v_V #v_A: Type0)
+      {| i0: Core_models.Cmp.t_Ord v_K |}
+      (self: t_BTreeMap v_K v_V v_A)
+      (key: v_K)
+      (value: v_V)
+    : Prims.Pure (t_BTreeMap v_K v_V v_A & Core_models.Option.t_Option v_V)
+      Prims.l_True
+      (fun _ -> Prims.l_True)
+
+/// See [`std::collections::BTreeMap::remove`]
+val impl_20__remove
+      (#v_K #v_V #v_A #v_Q: Type0)
+      {| i0: Core_models.Borrow.t_Borrow v_K v_Q |}
+      {| i1: Core_models.Cmp.t_Ord v_K |}
+      {| i2: Core_models.Cmp.t_Ord v_Q |}
+      (self: t_BTreeMap v_K v_V v_A)
+      (key: v_Q)
+    : Prims.Pure (t_BTreeMap v_K v_V v_A & Core_models.Option.t_Option v_V)
+      Prims.l_True
+      (fun _ -> Prims.l_True)
+
+/// See [`std::collections::BTreeMap::remove_entry`]
+val impl_20__remove_entry
+      (#v_K #v_V #v_A #v_Q: Type0)
+      {| i0: Core_models.Borrow.t_Borrow v_K v_Q |}
+      {| i1: Core_models.Cmp.t_Ord v_K |}
+      {| i2: Core_models.Cmp.t_Ord v_Q |}
+      (self: t_BTreeMap v_K v_V v_A)
+      (key: v_Q)
+    : Prims.Pure (t_BTreeMap v_K v_V v_A & Core_models.Option.t_Option (v_K & v_V))
+      Prims.l_True
+      (fun _ -> Prims.l_True)
+
+/// See [`std::collections::BTreeMap::append`]: on a shared key
+/// the value from `other` wins.
+val impl_20__append
+      (#v_K #v_V #v_A: Type0)
+      {| i0: Core_models.Cmp.t_Ord v_K |}
+      (self other: t_BTreeMap v_K v_V v_A)
+    : Prims.Pure (t_BTreeMap v_K v_V v_A & t_BTreeMap v_K v_V v_A)
+      Prims.l_True
+      (fun _ -> Prims.l_True)
+
+/// See [`std::collections::BTreeMap::split_off`]: keeps the
+/// entries with keys `< key`, returns those `>= key`.
+val impl_20__split_off
+      (#v_K #v_V #v_A #v_Q: Type0)
+      {| i0: Core_models.Borrow.t_Borrow v_K v_Q |}
+      {| i1: Core_models.Cmp.t_Ord v_K |}
+      {| i2: Core_models.Cmp.t_Ord v_Q |}
+      {| i3: Core_models.Clone.t_Clone v_A |}
+      (self: t_BTreeMap v_K v_V v_A)
+      (key: v_Q)
+    : Prims.Pure (t_BTreeMap v_K v_V v_A & t_BTreeMap v_K v_V v_A)
+      Prims.l_True
+      (fun _ -> Prims.l_True)
+
+/// See [`std::collections::BTreeMap::into_keys`]
+val impl_20__into_keys (#v_K #v_V #v_A: Type0) (self: t_BTreeMap v_K v_V v_A)
+    : Prims.Pure (t_IntoKeys v_K v_V v_A) Prims.l_True (fun _ -> Prims.l_True)
+
+/// See [`std::collections::BTreeMap::into_values`]
+val impl_20__into_values (#v_K #v_V #v_A: Type0) (self: t_BTreeMap v_K v_V v_A)
+    : Prims.Pure (t_IntoValues v_K v_V v_A) Prims.l_True (fun _ -> Prims.l_True)
+
+/// See [`std::collections::BTreeMap::len`]
+val impl_92__len (#v_K #v_V #v_A: Type0) (self: t_BTreeMap v_K v_V v_A)
+    : Prims.Pure usize Prims.l_True (fun _ -> Prims.l_True)
+
+/// See [`std::collections::BTreeMap::is_empty`]
+val impl_92__is_empty (#v_K #v_V #v_A: Type0) (self: t_BTreeMap v_K v_V v_A)
+    : Prims.Pure bool Prims.l_True (fun _ -> Prims.l_True)
+
+/// See [`std::collections::BTreeMap::iter`]
+val impl_92__iter (#v_K #v_V #v_A: Type0) (self: t_BTreeMap v_K v_V v_A)
+    : Prims.Pure (t_Iter v_K v_V) Prims.l_True (fun _ -> Prims.l_True)
+
+/// See [`std::collections::BTreeMap::keys`]
+val impl_92__keys (#v_K #v_V #v_A: Type0) (self: t_BTreeMap v_K v_V v_A)
+    : Prims.Pure (t_Keys v_K v_V) Prims.l_True (fun _ -> Prims.l_True)
+
+/// See [`std::collections::BTreeMap::values`]
+val impl_92__values (#v_K #v_V #v_A: Type0) (self: t_BTreeMap v_K v_V v_A)
+    : Prims.Pure (t_Values v_K v_V) Prims.l_True (fun _ -> Prims.l_True)
